Attempt at AES GCM decryption

specs/Spec.AESGCM.fst
@@ -12,7 +12,6 @@ let keylen: size_nat =   16
 let blocksize: size_nat = 16
 
 type key = lbytes keylen
-//type bytes = s:seq UInt8.t{length s < pow2 32}
 
 val ghash_:
   gmul_in_len:size_nat ->
@@ -39,7 +38,7 @@ let ghash text_len text aad_len aad tag_k k =
   (* TODO: rewrite with concat *)
   let aad_padding = (blocksize - (aad_len % blocksize)) % blocksize in
   let text_padding = (blocksize - (text_len % blocksize)) % blocksize in
-  let gmul_input_len:size_nat = aad_len + aad_padding + text_len + text_padding + blocksize in
+  let gmul_input_len: size_nat = aad_len + aad_padding + text_len + text_padding + blocksize in
   let gmul_input = create gmul_input_len (u8 0) in
   let gmul_input = update_slice gmul_input 0 aad_len aad  in
   let gmul_input = update_slice gmul_input (aad_len + aad_padding) (aad_len + aad_padding + text_len) text  in
@@ -58,10 +57,12 @@ val gcm:
   aad_len:size_nat ->
   aad:lbytes aad_len ->
   Tot Spec.GF128.tag
+
 let gcm k n_len n m_len m aad_len aad =
   let tag_key = AES.aes128_encrypt_bytes k n_len n 1 blocksize (create blocksize (u8 0)) in
   let mac = ghash m_len m aad_len aad tag_key k in
   mac
+
 
 val aead_encrypt:
   k:key ->
@@ -72,6 +73,7 @@ val aead_encrypt:
   aad_len:size_nat{(len + aad_len) / blocksize <= max_size_t} ->
   aad:lbytes aad_len ->
   Tot (lbytes (len + blocksize))
+
 let aead_encrypt k n_len n len m aad_len aad =
   let iv_len = if n_len = 12 then 12 else blocksize in
   let iv: lbytes iv_len = if n_len = 12 then n else (
@@ -92,3 +94,33 @@ let aead_encrypt k n_len n len m aad_len aad =
   let result = update_slice result 0 len c in
   let result = update_slice result len (len + blocksize) mac in
   result
+
+val aead_decrypt:
+  k:key ->
+  n_len:size_nat ->
+  n:lbytes n_len ->
+  len:size_nat ->
+  m:lbytes len ->
+  aad_len:size_nat{(len + aad_len) / blocksize <= max_size_t} ->
+  aad:lbytes aad_len ->
+  Tot (lbytes (len - blocksize))
+
+let aead_decrypt k n_len n len c aad_len aad =
+  let iv_len = if n_len = 12 then 12 else blocksize in
+  let iv: lbytes iv_len = if n_len = 12 then n else (
+    let n_padding:size_nat = (blocksize - (n_len % blocksize)) % blocksize in
+    let n_padding = n_padding + 8 in
+    let gmul_input_len = n_len + n_padding + 8 in
+    let gmul_input = create gmul_input_len (u8 0) in
+    let gmul_input = update_slice gmul_input 0 n_len n  in
+    let n_len_bytes = nat_to_bytes_be 8 (n_len * 8) in
+    let gmul_input = update_slice gmul_input (n_len + n_padding) (n_len + n_padding + 8) n_len_bytes  in
+    ghash_ gmul_input_len gmul_input (create blocksize (u8 0)) k
+  ) in
+  let computed_mac = gcm k iv_len iv len c aad_len aad in
+  let expected_mac = sub c (len - blocksize) blocksize in
+  let result = for_all2 (fun a b -> eq a b) computed_mac expected_mac in
+  if result then
+    AES.aes128_encrypt_bytes k iv_len iv 2 (len - blocksize) c
+  else
+    create blocksize (u8 0)
